assets/src/semantics-of-regular-expressions/Semantics.dfy
@@ -1,37 +1,27 @@
 include "Expressions.dfy"
 include "Languages.dfy"
 
-module Semantics {
-
-  import opened Expressions
-  import opened Languages
-
-  /* Definitions */
-
-  /* Denotational Semantics */
+module Semantics0 {
+  import opened Languages0
+  import opened Languages1
+  import opened Languages2
+  import opened Expressions0
 
   function Denotational<A(==)>(e: Exp): Lang {
     match e
-    case Zero => Languages.Zero()
-    case One => Languages.One()
-    case Char(a) => Languages.Singleton(a)
-    case Plus(e1, e2) => Languages.Plus(Denotational(e1), Denotational(e2))
-    case Comp(e1, e2) => Languages.Comp(Denotational(e1), Denotational(e2))
-    case Star(e1) => Languages.Star(Denotational(e1))
+    case Zero => Languages1.Zero()
+    case One => Languages2.One()
+    case Char(a) => Languages2.Singleton(a)
+    case Plus(e1, e2) => Languages2.Plus(Denotational(e1), Denotational(e2))
+    case Comp(e1, e2) => Languages2.Comp(Denotational(e1), Denotational(e2))
+    case Star(e1) => Languages2.Star(Denotational(e1))
   }
+}
 
-  /* Operational Semantics */
-
-  function Operational<A(==)>(e: Exp): Lang {
-    Alpha(Eps(e), (a: A) => Operational(Delta(e)(a)))
-  }
-
-  /* (Co)algebra homomorphisms f: Exp -> Lang */
-
-  ghost predicate IsCoalgebraHomomorphism<A(!new)>(f: Exp -> Lang) {
-    && (forall e :: f(e).eps == Eps(e))
-    && (forall e, a :: Bisimilar(f(e).delta(a), f(Delta(e)(a))))
-  }
+module Semantics1 {
+  import opened Languages0
+  import opened Languages3
+  import opened Expressions0
 
   ghost predicate IsAlgebraHomomorphism<A(!new)>(f: Exp -> Lang) {
     forall e :: IsAlgebraHomomorphismPointwise(f, e)
@@ -41,63 +31,20 @@ module Semantics {
     Bisimilar<A>(
       f(e),
       match e
-      case Zero => Languages.Zero()
-      case One => Languages.One()
-      case Char(a) => Languages.Singleton(a)
-      case Plus(e1, e2) => Languages.Plus(f(e1), f(e2))
-      case Comp(e1, e2) => Languages.Comp(f(e1), f(e2))
-      case Star(e1) => Languages.Star(f(e1))
+      case Zero => Languages1.Zero()
+      case One => Languages2.One()
+      case Char(a) => Languages2.Singleton(a)
+      case Plus(e1, e2) => Languages2.Plus(f(e1), f(e2))
+      case Comp(e1, e2) => Languages2.Comp(f(e1), f(e2))
+      case Star(e1) => Languages2.Star(f(e1))
     )
   }
+}
 
-  /* Lemmas */
-
-  /* Any two coalgebra homomorphisms f,g: Exp -> Lang are equal up to bisimulation */
-
-  lemma UniqueCoalgebraHomomorphism<A(!new)>(f: Exp -> Lang, g: Exp -> Lang, e: Exp)
-    requires IsCoalgebraHomomorphism(f)
-    requires IsCoalgebraHomomorphism(g)
-    ensures Bisimilar(f(e), g(e))
-  {
-    BisimilarityIsReflexive(f(e));
-    BisimilarityIsReflexive(g(e));
-    UniqueCoalgebraHomomorphismHelper(f, g, f(e), g(e));
-  }
-
-  lemma UniqueCoalgebraHomomorphismHelper<A(!new)>(f: Exp -> Lang, g: Exp -> Lang, L1: Lang, L2: Lang)
-    requires IsCoalgebraHomomorphism(f)
-    requires IsCoalgebraHomomorphism(g)
-    requires exists e :: Bisimilar(L1, f(e)) && Bisimilar(L2, g(e))
-    ensures Bisimilar(L1, L2)
-  {
-    forall k: nat
-      ensures Bisimilar#[k](L1, L2)
-    {
-      if k != 0 {
-        UniqueCoalgebraHomomorphismHelperPointwise(k, f, g, L1, L2);
-      }
-    }
-  }
-
-  lemma UniqueCoalgebraHomomorphismHelperPointwise<A(!new)>(k: nat, f: Exp -> Lang, g: Exp -> Lang, L1: Lang, L2: Lang)
-    requires IsCoalgebraHomomorphism(f)
-    requires IsCoalgebraHomomorphism(g)
-    requires exists e :: Bisimilar#[k](L1, f(e)) && Bisimilar#[k](L2, g(e))
-    ensures Bisimilar#[k](L1, L2)
-  {
-    var e :| Bisimilar#[k](L1, f(e)) && Bisimilar#[k](L2, g(e));
-    if k != 0 {
-      forall a
-        ensures Bisimilar#[k-1](L1.delta(a), L2.delta(a))
-      {
-        BisimilarityIsTransitivePointwise(k-1, L1.delta(a),  f(e).delta(a), f(Delta(e)(a)));
-        BisimilarityIsTransitivePointwise(k-1, L2.delta(a),  g(e).delta(a), g(Delta(e)(a)));
-        UniqueCoalgebraHomomorphismHelperPointwise(k-1, f, g, L1.delta(a), L2.delta(a));
-      }
-    }
-  }
-
-  /* Denotational is an algebra homomorphism */
+module Semantics2 {
+  import opened Semantics0
+  import opened Semantics1
+  import opened Languages4
 
   lemma DenotationalIsAlgebraHomomorphism<A(!new)>()
     ensures IsAlgebraHomomorphism<A>(Denotational)
@@ -108,8 +55,66 @@ module Semantics {
       BisimilarityIsReflexive<A>(Denotational(e));
     }
   }
+}
 
-  /* Denotational is a coalgebra homomorphism */
+module Semantics3 {
+  import opened Expressions0
+  import opened Expressions1
+  import opened Languages0
+
+  function Operational<A(==)>(e: Exp): Lang {
+    Alpha(Eps(e), (a: A) => Operational(Delta(e)(a)))
+  }
+}
+
+module Semantics4 {
+  import opened Expressions0
+  import opened Expressions1
+  import opened Languages0
+  import opened Languages3
+
+  ghost predicate IsCoalgebraHomomorphism<A(!new)>(f: Exp -> Lang) {
+    && (forall e :: f(e).eps == Eps(e))
+    && (forall e, a :: Bisimilar(f(e).delta(a), f(Delta(e)(a))))
+  }
+}
+
+module Semantics5 {
+  import opened Semantics3
+  import opened Semantics4
+  import opened Languages3
+  import opened Languages4
+  import opened Expressions1
+
+  lemma OperationalIsCoalgebraHomomorphism<A(!new)>()
+    ensures IsCoalgebraHomomorphism<A>(Operational)
+  {
+    forall e, a
+      ensures Bisimilar<A>(Operational(e).delta(a), Operational(Delta(e)(a)))
+    {
+      BisimilarityIsReflexive(Operational(e).delta(a));
+    }
+  }
+}
+
+module Semantics6 {
+  import opened Semantics0
+  import opened Semantics1
+  import opened Semantics2
+  import opened Semantics3
+  import opened Semantics4
+
+  lemma DenotationalIsCoalgebraHomomorphism<A(!new)>()
+    ensures IsCoalgebraHomomorphism<A>(Denotational)
+}
+
+module Semantics6WithProof refines Semantics6 {
+  import opened Expressions0
+  import opened Expressions1
+  import opened Languages0
+  import opened Languages3
+  import opened Languages4
+  import opened Languages5
 
   lemma DenotationalIsCoalgebraHomomorphism<A(!new)>()
     ensures IsCoalgebraHomomorphism<A>(Denotational)
@@ -147,13 +152,13 @@ module Semantics {
     ensures Bisimilar(Denotational<A>(e).delta(a), Denotational<A>(Delta(e)(a)))
   {
     match e
-    case Zero => BisimilarityIsReflexive<A>(Languages.Zero());
-    case One => BisimilarityIsReflexive<A>(Languages.One());
+    case Zero => BisimilarityIsReflexive<A>(Languages1.Zero());
+    case One => BisimilarityIsReflexive<A>(Languages2.One());
     case Char(b) =>
       if a == b {
-        BisimilarityIsReflexive<A>(Languages.One());
+        BisimilarityIsReflexive<A>(Languages2.One());
       } else {
-        BisimilarityIsReflexive<A>(Languages.Zero());
+        BisimilarityIsReflexive<A>(Languages1.Zero());
       }
     case Plus(e1, e2) =>
       DenotationalIsCoalgebraHomomorphismHelper2(e1, a);
@@ -164,7 +169,7 @@ module Semantics {
       DenotationalIsCoalgebraHomomorphismHelper2(e1, a);
       DenotationalIsCoalgebraHomomorphismHelper2(e2, a);
       BisimilarityIsReflexive<A>(Denotational(e2));
-      BisimilarityIsReflexive<A>(if Eps(e1) then Languages.One() else Languages.Zero());
+      BisimilarityIsReflexive<A>(if Eps(e1) then Languages2.One() else Languages1.Zero());
       CompCongruence(
         Denotational(e1).delta(a),
         Denotational(Delta(e1)(a)),
@@ -172,80 +177,114 @@ module Semantics {
         Denotational(e2)
       );
       CompCongruence(
-        if Eps(e1) then Languages.One() else Languages.Zero(),
-        if Eps(e1) then Languages.One() else Languages.Zero(),
+        if Eps(e1) then Languages2.One() else Languages1.Zero(),
+        if Eps(e1) then Languages2.One() else Languages1.Zero(),
         Denotational(e2).delta(a),
         Denotational(Delta(e2)(a))
       );
       PlusCongruence(
-        Languages.Comp(Denotational(e1).delta(a), Denotational(e2)),
-        Languages.Comp(Denotational(Delta(e1)(a)), Denotational(e2)),
-        Languages.Comp(if Eps(e1) then Languages.One() else Languages.Zero(), Denotational(e2).delta(a)),
-        Languages.Comp(if Eps(e1) then Languages.One() else Languages.Zero(), Denotational(Delta(e2)(a)))
+        Languages2.Comp(Denotational(e1).delta(a), Denotational(e2)),
+        Languages2.Comp(Denotational(Delta(e1)(a)), Denotational(e2)),
+        Languages2.Comp(if Eps(e1) then Languages2.One() else Languages1.Zero(), Denotational(e2).delta(a)),
+        Languages2.Comp(if Eps(e1) then Languages2.One() else Languages1.Zero(), Denotational(Delta(e2)(a)))
       );
     case Star(e1) =>
       DenotationalIsCoalgebraHomomorphismHelper2(e1, a);
-      BisimilarityIsReflexive(Languages.Star(Denotational(e1)));
-      CompCongruence(Denotational(e1).delta(a), Denotational(Delta(e1)(a)), Languages.Star(Denotational(e1)), Languages.Star(Denotational(e1)));
+      BisimilarityIsReflexive(Languages2.Star(Denotational(e1)));
+      CompCongruence(Denotational(e1).delta(a), Denotational(Delta(e1)(a)), Languages2.Star(Denotational(e1)), Languages2.Star(Denotational(e1)));
+  }
+}
+
+module Semantics7 {
+  import opened Expressions0
+  import opened Languages0
+  import opened Languages3
+  import opened Semantics4
+
+  lemma UniqueCoalgebraHomomorphism<A(!new)>(f: Exp -> Lang, g: Exp -> Lang, e: Exp)
+    requires IsCoalgebraHomomorphism(f)
+    requires IsCoalgebraHomomorphism(g)
+    ensures Bisimilar(f(e), g(e))
+}
+
+module Semantics7WithProof refines Semantics7 {
+  import opened Languages4
+  import opened Semantics8
+
+  lemma UniqueCoalgebraHomomorphism<A(!new)>(f: Exp<A> -> Lang<A>, g: Exp<A> -> Lang<A>, e: Exp<A>)
+    ensures Bisimilar(f(e), g(e))
+  {
+    BisimilarityIsReflexive(f(e));
+    BisimilarityIsReflexive(g(e));
+    UniqueCoalgebraHomomorphismHelper(f, g, f(e), g(e));
   }
 
-  /* Operational is an algebra homomorphism */
-
-  lemma OperationalIsAlgebraHomomorphism<A(!new)>()
-    ensures IsAlgebraHomomorphism<A>(Operational)
+  lemma UniqueCoalgebraHomomorphismHelper<A(!new)>(f: Exp -> Lang, g: Exp -> Lang, L1: Lang, L2: Lang)
+    requires IsCoalgebraHomomorphism(f)
+    requires IsCoalgebraHomomorphism(g)
+    requires exists e :: Bisimilar(L1, f(e)) && Bisimilar(L2, g(e))
+    ensures Bisimilar(L1, L2)
   {
-    forall e 
-      ensures IsAlgebraHomomorphismPointwise<A>(Operational, e) 
+    forall k: nat
+      ensures Bisimilar#[k](L1, L2)
     {
-      OperationalAndDenotationalAreBisimilar<A>(e);
-      assert IsAlgebraHomomorphismPointwise(Denotational, e) by {
-        DenotationalIsAlgebraHomomorphism<A>();
+      if k != 0 {
+        UniqueCoalgebraHomomorphismHelperPointwise(k, f, g, L1, L2);
       }
-      match e
-      case Zero =>
-        BisimilarityIsTransitive(Operational<A>(Zero), Denotational<A>(Zero), Languages.Zero());
-      case One =>
-        BisimilarityIsTransitive(Operational<A>(One), Denotational<A>(One), Languages.One());
-      case Char(a) =>
-        BisimilarityIsTransitive(Operational<A>(Char(a)), Denotational<A>(Char(a)), Languages.Singleton(a));
-      case Plus(e1, e2) =>
-        BisimilarityIsTransitive(Operational<A>(Plus(e1, e2)), Denotational<A>(Plus(e1, e2)), Languages.Plus(Denotational(e1), Denotational(e2)));
-        OperationalAndDenotationalAreBisimilar(e1);
-        BisimilarityIsSymmetric(Denotational(e1), Operational(e1));
-        OperationalAndDenotationalAreBisimilar(e2);
-        BisimilarityIsSymmetric(Denotational(e2), Operational(e2));
-        PlusCongruence<A>(Denotational(e1), Operational(e1), Denotational(e2), Operational(e2));
-        BisimilarityIsTransitive(Operational<A>(Plus(e1, e2)), Languages.Plus(Denotational(e1), Denotational(e2)), Languages.Plus(Operational(e1), Operational(e2)));
-      case Comp(e1, e2) =>
-        BisimilarityIsTransitive(Operational<A>(Comp(e1, e2)), Denotational<A>(Comp(e1, e2)), Languages.Comp(Denotational(e1), Denotational(e2)));
-        OperationalAndDenotationalAreBisimilar(e1);
-        BisimilarityIsSymmetric(Denotational(e1), Operational(e1));
-        OperationalAndDenotationalAreBisimilar(e2);
-        BisimilarityIsSymmetric(Denotational(e2), Operational(e2));
-        CompCongruence<A>(Denotational(e1), Operational(e1), Denotational(e2), Operational(e2));
-        BisimilarityIsTransitive(Operational<A>(Comp(e1, e2)), Languages.Comp(Denotational(e1), Denotational(e2)), Languages.Comp(Operational(e1), Operational(e2)));
-      case Star(e1) =>
-        BisimilarityIsTransitive(Operational<A>(Star(e1)), Denotational<A>(Star(e1)), Languages.Star(Denotational(e1)));
-        OperationalAndDenotationalAreBisimilar(e1);
-        BisimilarityIsSymmetric(Denotational(e1), Operational(e1));
-        StarCongruence(Denotational(e1), Operational(e1));
-        BisimilarityIsTransitive(Operational<A>(Star(e1)), Languages.Star(Denotational(e1)), Languages.Star(Operational(e1)));
     }
   }
+}
 
-  /* Operational is a coalgebra homomorphism */
+module Semantics8 {
+  import opened Expressions0
+  import opened Expressions1
+  import opened Languages0
+  import opened Languages3
+  import opened Semantics4
 
-  lemma OperationalIsCoalgebraHomomorphism<A(!new)>()
-    ensures IsCoalgebraHomomorphism<A>(Operational)
+  lemma UniqueCoalgebraHomomorphismHelperPointwise<A(!new)>(k: nat, f: Exp -> Lang, g: Exp -> Lang, L1: Lang, L2: Lang)
+    requires IsCoalgebraHomomorphism(f)
+    requires IsCoalgebraHomomorphism(g)
+    requires exists e :: Bisimilar#[k](L1, f(e)) && Bisimilar#[k](L2, g(e))
+    ensures Bisimilar#[k](L1, L2)
   {
-    forall e, a
-      ensures Bisimilar<A>(Operational(e).delta(a), Operational(Delta(e)(a)))
-    {
-      BisimilarityIsReflexive(Operational(e).delta(a));
+    var e :| Bisimilar#[k](L1, f(e)) && Bisimilar#[k](L2, g(e));
+    if k != 0 {
+      forall a
+        ensures Bisimilar#[k-1](L1.delta(a), L2.delta(a))
+      {
+        BisimilarityIsTransitivePointwise(k-1, L1.delta(a),  f(e).delta(a), f(Delta(e)(a)));
+        BisimilarityIsTransitivePointwise(k-1, L2.delta(a),  g(e).delta(a), g(Delta(e)(a)));
+        UniqueCoalgebraHomomorphismHelperPointwise(k-1, f, g, L1.delta(a), L2.delta(a));
+      }
     }
   }
 
-  /* Operational and Denotational are equal, up to bisimulation */
+  lemma BisimilarityIsTransitivePointwise<A(!new)>(k: nat, L1: Lang, L2: Lang, L3: Lang)
+    ensures Bisimilar#[k](L1, L2) && Bisimilar#[k](L2, L3) ==> Bisimilar#[k](L1, L3)
+  {
+    if k != 0 {
+      if Bisimilar#[k](L1, L2) && Bisimilar#[k](L2, L3) {
+        assert Bisimilar#[k](L1, L3) by {
+          forall a
+            ensures Bisimilar#[k-1](L1.delta(a), L3.delta(a))
+          {
+            BisimilarityIsTransitivePointwise(k-1, L1.delta(a), L2.delta(a), L3.delta(a));
+          }
+        }
+      }
+    }
+  }
+}
+
+module Semantics9 {
+  import opened Expressions0
+  import opened Languages3
+  import opened Semantics5
+  import opened Semantics0
+  import opened Semantics3
+  import opened Semantics6WithProof
+  import opened Semantics7WithProof
 
   lemma OperationalAndDenotationalAreBisimilar<A(!new)>(e: Exp)
     ensures Bisimilar<A>(Operational(e), Denotational(e))
@@ -254,5 +293,66 @@ module Semantics {
     DenotationalIsCoalgebraHomomorphism<A>();
     UniqueCoalgebraHomomorphism<A>(Operational, Denotational, e);
   }
+}
 
+module Semantics10 {
+  import opened Semantics1
+  import opened Semantics3
+
+  lemma OperationalIsAlgebraHomomorphism<A(!new)>()
+    ensures IsAlgebraHomomorphism<A>(Operational)
+}
+
+module Semantics10WithProof refines Semantics10 {
+  import opened Expressions0
+  import opened Semantics0
+  import opened Semantics2
+  import opened Semantics9
+  import opened Languages1
+  import opened Languages2
+  import opened Languages6
+  import opened Languages5
+  import opened Languages7
+
+  lemma OperationalIsAlgebraHomomorphism<A(!new)>()
+    ensures IsAlgebraHomomorphism<A>(Operational)
+  {
+    forall e
+      ensures IsAlgebraHomomorphismPointwise<A>(Operational, e)
+    {
+      OperationalAndDenotationalAreBisimilar<A>(e);
+      assert IsAlgebraHomomorphismPointwise(Denotational, e) by {
+        DenotationalIsAlgebraHomomorphism<A>();
+      }
+      match e
+      case Zero =>
+        BisimilarityIsTransitive(Operational<A>(Zero), Denotational<A>(Zero), Languages1.Zero());
+      case One =>
+        BisimilarityIsTransitive(Operational<A>(One), Denotational<A>(One), Languages2.One());
+      case Char(a) =>
+        BisimilarityIsTransitive(Operational<A>(Char(a)), Denotational<A>(Char(a)), Languages2.Singleton(a));
+      case Plus(e1, e2) =>
+        BisimilarityIsTransitive(Operational<A>(Plus(e1, e2)), Denotational<A>(Plus(e1, e2)), Languages2.Plus(Denotational(e1), Denotational(e2)));
+        OperationalAndDenotationalAreBisimilar(e1);
+        BisimilarityIsSymmetric(Denotational(e1), Operational(e1));
+        OperationalAndDenotationalAreBisimilar(e2);
+        BisimilarityIsSymmetric(Denotational(e2), Operational(e2));
+        PlusCongruence<A>(Denotational(e1), Operational(e1), Denotational(e2), Operational(e2));
+        BisimilarityIsTransitive(Operational<A>(Plus(e1, e2)), Languages2.Plus(Denotational(e1), Denotational(e2)), Languages2.Plus(Operational(e1), Operational(e2)));
+      case Comp(e1, e2) =>
+        BisimilarityIsTransitive(Operational<A>(Comp(e1, e2)), Denotational<A>(Comp(e1, e2)), Languages2.Comp(Denotational(e1), Denotational(e2)));
+        OperationalAndDenotationalAreBisimilar(e1);
+        BisimilarityIsSymmetric(Denotational(e1), Operational(e1));
+        OperationalAndDenotationalAreBisimilar(e2);
+        BisimilarityIsSymmetric(Denotational(e2), Operational(e2));
+        CompCongruence<A>(Denotational(e1), Operational(e1), Denotational(e2), Operational(e2));
+        BisimilarityIsTransitive(Operational<A>(Comp(e1, e2)), Languages2.Comp(Denotational(e1), Denotational(e2)), Languages2.Comp(Operational(e1), Operational(e2)));
+      case Star(e1) =>
+        BisimilarityIsTransitive(Operational<A>(Star(e1)), Denotational<A>(Star(e1)), Languages2.Star(Denotational(e1)));
+        OperationalAndDenotationalAreBisimilar(e1);
+        BisimilarityIsSymmetric(Denotational(e1), Operational(e1));
+        StarCongruence(Denotational(e1), Operational(e1));
+        BisimilarityIsTransitive(Operational<A>(Star(e1)), Languages2.Star(Denotational(e1)), Languages2.Star(Operational(e1)));
+    }
+  }
 }
